@prefix core: <https://unifiedcyberontology.org/ontology/uco/core#> .
@prefix observable: <https://unifiedcyberontology.org/ontology/uco/observable#> .
@prefix drafting: <http://example.org/ontology/drafting#> .
@prefix owl: <http://www.w3.org/2002/07/owl#> .
@prefix rdf: <http://www.w3.org/1999/02/22-rdf-syntax-ns#> .
@prefix rdfs: <http://www.w3.org/2000/01/rdf-schema#> .
@prefix sh: <http://www.w3.org/ns/shacl#> .
@prefix xsd: <http://www.w3.org/2001/XMLSchema#> .

drafting:CellSiteFacet
	a
		sh:NodeShape ,
		owl:Class
		;
	rdfs:subClassOf core:Facet ;
	rdfs:seeAlso <https://case.atlassian.net/browse/ONT-469> ;
	rdfs:label "CellSiteFacet"@en ;
	rdfs:comment "A cell site facet contains the metadata surrounding the cell site."@en ;
	sh:property
		[
			sh:datatype xsd:string ;
			sh:maxCount "1"^^xsd:integer ;
			sh:nodeKind sh:Literal ;
			sh:path drafting:cellSiteType ;
		] ,		[
			sh:datatype xsd:string ;
			sh:maxCount "1"^^xsd:integer ;
			sh:nodeKind sh:Literal ;
			sh:path drafting:cellSiteIdentifier ;
		] ,
		[
			sh:datatype xsd:string ;
			sh:maxCount "1"^^xsd:integer ;
			sh:nodeKind sh:Literal ;
			sh:path drafting:cellSiteLocationAreaCode ;
		] ,
		[
			sh:datatype xsd:string ;
			sh:maxCount "1"^^xsd:integer ;
			sh:nodeKind sh:Literal ;
			sh:path drafting:cellSiteCountryCode ;
		] ,
		[
			sh:datatype xsd:string ;
			sh:maxCount "1"^^xsd:integer ;
			sh:nodeKind sh:Literal ;
			sh:path drafting:cellSiteNetworkCode ;
		]
		;
	sh:targetClass observable:CellSiteFacet ;
	.

drafting:AntennaFacet
	a
		owl:Class ,
		sh:NodeShape
		;
	rdfs:subClassOf core:Facet ;
	rdfs:seeAlso <https://case.atlassian.net/browse/ONT-469> ;
	rdfs:label "AntennaFacet"@en ;
	rdfs:comment "An antenna alignment facet contains the metadata surrounding the cell tower's antenna position."@en ;
	sh:property
		[
			sh:datatype xsd:decimal ;
			sh:maxCount "1"^^xsd:integer ;
			sh:nodeKind sh:Literal ;
			sh:path drafting:azimuth ;
		] ,
		[
			sh:datatype xsd:decimal ;
			sh:maxCount "1"^^xsd:integer ;
			sh:nodeKind sh:Literal ;
			sh:path drafting:elevation ;
		] ,
		[
			sh:datatype xsd:decimal ;
			sh:maxCount "1"^^xsd:integer ;
			sh:nodeKind sh:Literal ;
			sh:path drafting:signalStrength ;
		] ,
		[
			sh:datatype xsd:decimal ;
			sh:maxCount "1"^^xsd:integer ;
			sh:nodeKind sh:Literal ;
			sh:path drafting:horizontalBeamWidth ;
		] ,
		[
			sh:datatype xsd:decimal ;
			sh:maxCount "1"^^xsd:integer ;
			sh:nodeKind sh:Literal ;
			sh:path drafting:skew ;
		]
		;
	sh:targetClass observable:AntennaFacet ;
	.

drafting:CapturedTelecommunicationsInformationFacet
	a
		owl:Class ,
		sh:NodeShape
		;
	rdfs:subClassOf core:Facet ;
	rdfs:seeAlso <https://case.atlassian.net/browse/ONT-469> ;
	rdfs:label "CapturedTelecommunicationsInformationFacet"@en ;
	rdfs:comment "A captured telecommunications information facet represents certain information within captured or intercepted telecommunications data."@en ;
	sh:property
		[
			sh:class drafting:CellSite ;
			sh:maxCount "1"^^xsd:integer ;
			sh:minCount "1"^^xsd:integer ;
			sh:nodeKind sh:BlankNodeOrIRI ;
			sh:path drafting:captureCellSite ;
		] ,
		[
			sh:datatype xsd:dateTime ;
			sh:maxCount "1"^^xsd:integer ;
			sh:nodeKind sh:Literal ;
			sh:path observable:endTime ;
		] ,
		[
			sh:datatype xsd:string ;
			sh:maxCount "1"^^xsd:integer ;
			sh:nodeKind sh:Literal ;
			sh:path drafting:interceptedCallState ;
		] ,
		[
			sh:class observable:Device ;
			sh:nodeKind sh:Literal ;
			sh:path drafting:partyDevice ;
		] ,
		[
			sh:class observable:ObservableObject ;
			sh:nodeKind sh:Literal ;
			sh:path drafting:partySubscription ;
		] ,
		[
			sh:datatype xsd:dateTime ;
			sh:maxCount "1"^^xsd:integer ;
			sh:nodeKind sh:Literal ;
			sh:path observable:startTime ;
		]
		;
	sh:targetClass observable:CapturedTelecommunicationsInformationFacet ;
	.

drafting:azimuth
	a owl:DatatypeProperty ;
	rdfs:label "azimuth"@en ;
	rdfs:comment "The median rotation in degrees around a vertical axis of the cell antenna sector accessed."@en ;
	rdfs:range xsd:decimal ;
	.

drafting:captureCellSite
	a owl:ObjectProperty ;
	rdfs:label "captureCellTower"@en ;
	rdfs:comment "Specifies the cell site accessed."@en ;
	rdfs:range drafting:CellTower ;
	.

drafting:elevation
	a owl:DatatypeProperty ;
	rdfs:label "elevation"@en ;
	rdfs:comment "The angle in degrees of the antenna from the local horizontal plane."@en ;
	rdfs:range xsd:decimal ;
	.

drafting:interceptedCallState
	a owl:DatatypeProperty ;
	rdfs:label "interceptedCallState"@en ;
	rdfs:comment "State of the call in a Call Detail Record (e.g. idle)."@en ;
	rdfs:range xsd:string ;
	.

drafting:partyDevice
	a owl:ObjectProperty ;
	rdfs:label "partyDevice"@en ;
	rdfs:comment "A device connected to the cell tower."@en ;
	rdfs:range observable:Device ;
	.

drafting:partySubscription
	a owl:ObjectProperty ;
	rdfs:label "partySubscription"@en ;
	rdfs:comment "The addresses of the device connected to the cell tower (references IMSI, MSISDN SIP address, 5G supi)."@en ;
	rdfs:range observable:ObservableObject ;
	.

drafting:skew
	a owl:DatatypeProperty ;
	rdfs:label "skew"@en ;
	rdfs:comment "The angle in degrees of the radial rotation around its main beam direction."@en ;
	rdfs:range xsd:decimal ;
	.

drafting:cellSiteType
	a owl:DatatypeProperty ;
	rdfs:label "cellSiteType"@en ;
	rdfs:comment "Specifies the technology used by the Cell Site (e.g., GSM, CDMA, or LTE)."@en ;
	rdfs:range xsd:string ;
	.

drafting:cellSiteIdentifier
	a owl:DatatypeProperty ;
	rdfs:label "cellSiteIdentifier"@en ;
	rdfs:comment "Specifies the unique number used to identify each Cell Site within a location area code."@en ;
	rdfs:range xsd:string ;
	.
	
drafting:cellSiteLocationAreaCode
	a owl:DatatypeProperty ;
	rdfs:label "cellSiteLocationAreaCode"@en ;
	rdfs:comment "The location area code is a unique number of current location area of the cell site. A location area is a set of cell site that are grouped together to optimize signalling. For GSM, this is the LAC."@en ;
	rdfs:range xsd:string ;
	.

drafting:cellSiteCountryCode
	a owl:DatatypeProperty ;
	rdfs:label "cellSiteCountryCode"@en ;
	rdfs:comment "The country code represents the country of the cell site. For GSM, this is the Mobile Country Code (MCC)."@en ;
	rdfs:range xsd:string ;
	.

drafting:cellSiteNetworkCode
	a owl:DatatypeProperty ;
	rdfs:label "cellSiteNetworkCode"@en ;
	rdfs:comment "The this code identifies the mobile operator of the cell site. For GSM, this is the Mobile Network Code (MNC) and for CMDA this is the network identifier (NID)."@en ;
	rdfs:range xsd:string ;
	.

drafting:signalStrength
	a owl:DatatypeProperty ;
	rdfs:label "signalStrength"@en ;
	rdfs:comment "The strength of the antenna signal."@en ;
	rdfs:range xsd:string ;
	.

drafting:horizontalBeamWidth
	a owl:DatatypeProperty ;
	rdfs:label "horizontalBeamWidth"@en ;
	rdfs:comment "The width of the antenna beam in degrees."@en ;
	rdfs:range xsd:string ;
	.

