@prefix core: <https://unifiedcyberontology.org/ontology/uco/core#> .
@prefix observable: <https://unifiedcyberontology.org/ontology/uco/observable#> .
@prefix drafting: <http://example.org/ontology/drafting#> .
@prefix owl: <http://www.w3.org/2002/07/owl#> .
@prefix rdf: <http://www.w3.org/1999/02/22-rdf-syntax-ns#> .
@prefix rdfs: <http://www.w3.org/2000/01/rdf-schema#> .
@prefix sh: <http://www.w3.org/ns/shacl#> .
@prefix xsd: <http://www.w3.org/2001/XMLSchema#> .

drafting:CellTowerFacet
	a
		sh:NodeShape ,
		owl:Class
		;
	rdfs:subClassOf core:Facet ;
	rdfs:seeAlso <case.atlassian.net/browse/ONT-469> ;
	rdfs:label "CellTowerFacet"@en ;
	rdfs:comment "A cell tower facet contains the metadata surrounding the cell tower."@en ;
	sh:property
		[
			sh:datatype xsd:string ;
			sh:maxCount "1"^^xsd:integer ;
			sh:nodeKind sh:Literal ;
			sh:path drafting:towerCid ;
		] ,
		[
			sh:datatype xsd:string ;
			sh:maxCount "1"^^xsd:integer ;
			sh:nodeKind sh:Literal ;
			sh:path drafting:towerLac ;
		] ,
		[
			sh:datatype xsd:string ;
			sh:maxCount "1"^^xsd:integer ;
			sh:nodeKind sh:Literal ;
			sh:path drafting:towerMcc ;
		] ,
		[
			sh:datatype xsd:string ;
			sh:maxCount "1"^^xsd:integer ;
			sh:nodeKind sh:Literal ;
			sh:path drafting:towerMnc ;
		]
		;
	sh:targetClass observable:CellTowerFacet ;
	.

drafting:AntennaAlignmentFacet
	a
		owl:Class ,
		sh:NodeShape
		;
	rdfs:subClassOf core:Facet ;
	rdfs:seeAlso <case.atlassian.net/browse/ONT-469> ;
	rdfs:label "AntennaAlignmentFacet"@en ;
	rdfs:comment "An antenna alignment facet contains the metadata surrounding the cell tower's antenna position."@en ;
	sh:property
		[
			sh:datatype xsd:decimal ;
			sh:maxCount "1"^^xsd:integer ;
			sh:nodeKind sh:Literal ;
			sh:path drafting:azimuth ;
		] ,
		[
			sh:datatype xsd:decimal ;
			sh:maxCount "1"^^xsd:integer ;
			sh:nodeKind sh:Literal ;
			sh:path drafting:elevation ;
		] ,
		[
			sh:datatype xsd:decimal ;
			sh:maxCount "1"^^xsd:integer ;
			sh:nodeKind sh:Literal ;
			sh:path drafting:skew ;
		]
		;
	sh:targetClass observable:AntennaAlignmentFacet ;
	.

drafting:CapturedTelecommunicationsInformationFacet
	a
		owl:Class ,
		sh:NodeShape
		;
	rdfs:subClassOf core:Facet ;
	rdfs:seeAlso <case.atlassian.net/browse/ONT-469> ;
	rdfs:label "CapturedTelecommunicationsInformationFacet"@en ;
	rdfs:comment "A captured telecommunications information facet represents certain information within captured or intercepted telecommunications data."@en ;
	sh:property
		[
			sh:class observable:ObservableObject
			sh:maxCount "1"^^xsd:integer ;
			sh:minCount "1"^^xsd:integer ;
			sh:nodeKind sh:BlankNodeOrIRI ;
			sh:path drafting:captureCellTower ;
		] ,
		[
			sh:datatype xsd:dateTime ;
			sh:maxCount "1"^^xsd:integer ;
			sh:nodeKind sh:Literal ;
			sh:path observable:endTime ;
		] ,
		[
			sh:datatype xsd:string ;
			sh:maxCount "1"^^xsd:integer ;
			sh:nodeKind sh:Literal ;
			sh:path drafting:interceptedCallState ;
		] ,
		[
			sh:class observable:ObservableObject
			sh:nodeKind sh:Literal ;
			sh:path drafting:partyDevice ;
		] ,
		[
			sh:class observable:ObservableObject
			sh:nodeKind sh:Literal ;
			sh:path drafting:partySubscription ;
		] ,
		[
			sh:datatype xsd:dateTime ;
			sh:maxCount "1"^^xsd:integer ;
			sh:nodeKind sh:Literal ;
			sh:path observable:startTime ;
		]
		;
	sh:targetClass observable:CapturedTelecommunicationsInformationFacet ;
	.

drafting:azimuth
	a owl:DatatypeProperty ;
	rdfs:label "azimuth"@en ;
	rdfs:comment "The median rotation in degrees around a vertical axis of the cell antenna sector accessed."@en ;
	rdfs:range xsd:decimal ;
	.

drafting:captureCellTower
	a owl:ObjectProperty ;
	rdfs:label "captureCellTower"@en ;
	rdfs:comment "Specifies the cell tower accessed."@en ;
	rdfs:range observable:ObservableObject ;
	.

drafting:elevation
	a owl:DatatypeProperty ;
	rdfs:label "elevation"@en ;
	rdfs:comment "The angle in degrees of the antenna from the local horizontal plane."@en ;
	rdfs:range xsd:decimal ;
	.

drafting:interceptedCallState
	a owl:DatatypeProperty ;
	rdfs:label "interceptedCallState"@en ;
	rdfs:comment "State of the call in a Call Detail Record (e.g. idle)."@en ;
	rdfs:range xsd:string ;
	.

drafting:partyDevice
	a owl:ObjectProperty ;
	rdfs:label "partyDevice"@en ;
	rdfs:comment "The IMEI of the device connected to the cell tower."@en ;
	rdfs:range observable:ObservableObject ;
	.

drafting:partySubscription
	a owl:ObjectProperty ;
	rdfs:label "partySubscription"@en ;
	rdfs:comment "The addresses of the device connected to the cell tower (references IMSI, MSISDN SIP address, 5G supi)."@en ;
	rdfs:range observable:ObservableObject ;
	.

drafting:skew
	a owl:DatatypeProperty ;
	rdfs:label "skew"@en ;
	rdfs:comment "The angle in degrees of the radial rotation around its main beam direction."@en ;
	rdfs:range xsd:decimal ;
	.

drafting:towerBid
	a owl:DatatypeProperty ;
	rdfs:label "towerBid"@en ;
	rdfs:comment "Specifies the BID segment of the CDMA identifier of the cell tower."@en ;
	rdfs:range xsd:string ;
	.

drafting:towerCid
	a owl:DatatypeProperty ;
	rdfs:label "towerCid"@en ;
	rdfs:comment "Specifies the global identifier network code of the cell tower."@en ;
	rdfs:range xsd:string ;
	.
	
drafting:towerLac
	a owl:DatatypeProperty ;
	rdfs:label "towerLac"@en ;
	rdfs:comment "The Location Area Code (LAC) is a fixed length code (of 2 octets) identifying a location area within a PLMN."@en ;
	rdfs:range xsd:string ;
	.

drafting:towerMcc
	a owl:DatatypeProperty ;
	rdfs:label "towerMcc"@en ;
	rdfs:comment "The Mobile Country Code (MCC) is a three digit code representing the country of the cell tower."@en ;
	rdfs:range xsd:string ;
	.

drafting:towerMnc
	a owl:DatatypeProperty ;
	rdfs:label "towerMnc"@en ;
	rdfs:comment "The Mobile Network Code (MNC) is a two or three digit code representing the network of the cell tower."@en ;
	rdfs:range xsd:string ;
	.

drafting:towerNid
	a owl:DatatypeProperty ;
	rdfs:label "towerNid"@en ;
	rdfs:comment "Specifies the NID segment of the CDMA identifier of the cell tower."@en ;
	rdfs:range xsd:string ;
	.

drafting:towerSid
	a owl:DatatypeProperty ;
	rdfs:label "towerSid"@en ;
	rdfs:comment "Specifies the SID segment of the CDMA identifier of the cell tower."@en ;
	rdfs:range xsd:string ;
	.

drafting:towerType
	a owl:DatatypeProperty ;
	rdfs:label "towerType"@en ;
	rdfs:comment "Specifies the network type of the cell tower (GSM, CDMA, etc)."@en ;
	rdfs:range xsd:string ;
	.