@prefix drafting: <http://example.org/ontology/drafting/> .
@prefix owl: <http://www.w3.org/2002/07/owl#> .
@prefix rdf: <http://www.w3.org/1999/02/22-rdf-syntax-ns#> .
@prefix rdfs: <http://www.w3.org/2000/01/rdf-schema#> .
@prefix uco-core: <https://unifiedcyberontology.org/ontology/uco/core#> .
@prefix xsd: <http://www.w3.org/2001/XMLSchema#> .

drafting:Hypothesis
	a owl:Class ;
	rdfs:subClassOf uco-core:Assertion ;
	rdfs:label "Hypothesis"@en ;
	rdfs:comment "A natural-language claim to explain observable objects."@en ;
	rdfs:seeAlso <https://case.atlassian.net/browse/ONT-434> ;
	.

drafting:Inference
	a owl:Class ;
	rdfs:subClassOf
		uco-core:UcoObject ,
		[
			a owl:Restriction ;
			owl:onProperty drafting:evidenceEvaluation ;
			owl:maxQualifiedCardinality "1"^^xsd:nonNegativeInteger ;
			owl:onDataRange xsd:float ;
		] ,
		[
			a owl:Restriction ;
			owl:onProperty drafting:evaluationRationale ;
			owl:maxQualifiedCardinality "1"^^xsd:nonNegativeInteger ;
			owl:onDataRange xsd:string ;
		] ,
		[
			a owl:Restriction ;
			owl:onProperty drafting:evaluationType ;
			owl:maxQualifiedCardinality "1"^^xsd:nonNegativeInteger ;
			owl:onDataRange xsd:string ;
		] ,
		[
			a owl:Restriction ;
			owl:onProperty drafting:basisEvidence ;
			owl:onClass uco-core:UcoObject ;
			owl:minQualifiedCardinality "1"^^xsd:nonNegativeInteger ;
		] ,
		[
			a owl:Restriction ;
			owl:onProperty drafting:usedMethod ;
			owl:onClass drafting:Method ;
			owl:qualifiedCardinality "1"^^xsd:nonNegativeInteger ;
		] ,
		[
			a owl:Restriction ;
			owl:onProperty drafting:hypothesis ;
			owl:onDataRange xsd:string ;
			owl:qualifiedCardinality "1"^^xsd:nonNegativeInteger ;
		]
		;
	rdfs:label "Inference"@en ;
	rdfs:comment "An opinion that is formed on the basis of observed objects (evidence) in light of a given hypothesis." ;
	rdfs:seeAlso <https://case.atlassian.net/browse/ONT-434> ;
	.

drafting:Method
	a owl:Class ;
	rdfs:subClassOf uco-core:UcoObject ;
	rdfs:label "Method"@en ;
	rdfs:comment
		"(TODO - would this relate to Pattern?)"@en ,
		"A method is an interpretation algorithm or procedure."@en
		;
	rdfs:seeAlso <https://case.atlassian.net/browse/ONT-434> ;
	.

drafting:basisEvidence
	a owl:ObjectProperty ;
	rdfs:label "basisEvidence"@en ;
	rdfs:comment "Observed object(s) being evaluated as support for an inference." ;
	rdfs:range uco-core:UcoObject ;
	rdfs:seeAlso <https://case.atlassian.net/browse/ONT-434> ;
	.

drafting:evaluationRationale
	a owl:DatatypeProperty ;
	rdfs:label "evaluationRationale"@en ;
	rdfs:comment "Explanation of the rationale for an assigned number"@en ;
	rdfs:range xsd:string ;
	rdfs:seeAlso <https://case.atlassian.net/browse/ONT-434> ;
	.

drafting:evaluationType
	a owl:DatatypeProperty ;
	rdfs:label "evaluationType"@en ;
	rdfs:comment "What an assigned number represents such as probability, strength, similarity, etc."@en ;
	rdfs:range xsd:string ;
	rdfs:seeAlso <https://case.atlassian.net/browse/ONT-434> ;
	.

drafting:evidenceEvaluation
	a owl:DatatypeProperty ;
	rdfs:label "evidenceEvaluation"@en ;
	rdfs:comment
		"(TODO This should probably go into UCO Core.)"@en ,
		"A number that represents the probability, strength, similarity, etc. of the observed object(s) in light of the hypothesis."@en
		;
	rdfs:range xsd:float ;
	rdfs:seeAlso <https://case.atlassian.net/browse/ONT-434> ;
	.

drafting:hypothesis
	a owl:DatatypeProperty ;
	rdfs:label "hypothesis"@en ;
	rdfs:comment "A proposed explanation made on the basis of initial observations as a starting point for further investigation."@en ;
	rdfs:range xsd:string ;
	rdfs:seeAlso <https://case.atlassian.net/browse/ONT-434> ;
	.

drafting:usedMethod
	a owl:ObjectProperty ;
	rdfs:label "usedMethod"@en ;
	rdfs:comment "The process/algorithm used to assign a value to the observed evidence such as probability model, computed similarity (e.g., Levenshtein distance), strength of evidence (e.g. C-Scale)." ;
	rdfs:range drafting:Method ;
	rdfs:seeAlso <https://case.atlassian.net/browse/ONT-434> ;
	.

